src/Denote.v
@@ -20,12 +20,12 @@ Generalizable All Variables.
 
 Section Denote.
 
-Import EqNotations.
-
 Context {C : Category}.
 
 Variable objs : obj_idx -> C.
 Variable arrs : ∀ f : arr_idx, option (∃ x y, objs x ~{C}~> objs y).
+
+Import EqNotations.
 
 Fixpoint termD dom cod (e : Term) : option (objs dom ~{C}~> objs cod) :=
   match e with
@@ -35,7 +35,6 @@ Fixpoint termD dom cod (e : Term) : option (objs dom ~{C}~> objs cod) :=
         Some (rew [fun x => objs x ~{ C }~> objs cod] edom in @id _ (objs cod))
       | right _ => None
       end
-  (* jww (2017-08-02): Why does morph need [obj_idx] arguments? *)
   | Morph _ _ a =>
     match arrs a with
     | Some (x'; (y'; f)) =>
@@ -52,6 +51,17 @@ Fixpoint termD dom cod (e : Term) : option (objs dom ~{C}~> objs cod) :=
     | Some f, Some g => Some (f ∘ g)
     | _, _ => None
     end
+  end.
+
+Fixpoint exprD (e : Expr) : Type :=
+  match e with
+  | Top           => True
+  | Bottom        => False
+  | Equiv x y f g => termD x y f ≈ termD x y g
+  (* | Not p         => exprD p -> False *)
+  | And p q       => exprD p ∧ exprD q
+  | Or p q        => exprD p + exprD q
+  | Impl p q      => exprD p -> exprD q
   end.
 
 Fixpoint arrowsD dom cod `(fs : list (Arrow t)) :
@@ -92,114 +102,6 @@ Fixpoint arrowsD dom cod `(fs : list (Arrow t)) :
     end
   end.
 
-(*
-Lemma arrowsD_app x y m f1 f2 f g :
-  arrowsD m y (arrows f1) = Some f ->
-  arrowsD x m (arrows f2) = Some g ->
-  arrowsD x y (arrows (Compose m f1 f2)) ≈ Some (f ∘ g).
-Proof.
-  intros.
-  generalize dependent f2.
-  generalize dependent f.
-  generalize dependent g.
-  generalize dependent m.
-  generalize dependent y.
-  generalize dependent x.
-  induction f1; simpl; intros; equalities.
-  - inversion_clear H.
-    admit.
-  - destruct (arrs _); [|discriminate].
-    destruct s, s; repeat equalities.
-Admitted.
-
-Lemma arrowsD_termD_some x y f r :
-  arrowsD x y (arrows f) = Some r -> termD x y f ≈ Some r.
-Proof.
-  generalize dependent r.
-  generalize dependent y.
-  generalize dependent x.
-  induction f; simpl; intros; repeat equalities; simpl_eq.
-  - inversion_clear H; cat.
-  - destruct (arrs _); [|discriminate].
-    destruct s, s; equalities.
-    equalities'; auto.
-    equalities'; auto.
-    equalities; [|discriminate].
-    inversion_clear H.
-    reflexivity.
-  - rewrite arrowsD_app in H.
-    equalities.
-    specialize (IHf1 _ _ _ a).
-    specialize (IHf2 _ _ _ a0).
-    destruct (termD m y f1) eqn:?, (termD x m f2) eqn:?; try tauto.
-    red in IHf1.
-    red in IHf2.
-    rewrite IHf1, IHf2, b0.
-    reflexivity.
-Qed.
-
-Lemma termD_arrowsD_some x y f r :
-  termD x y f = Some r -> arrowsD x y (arrows f) ≈ Some r.
-Proof.
-  generalize dependent r.
-  generalize dependent y.
-  generalize dependent x.
-  induction f; simpl; intros; repeat equalities; simpl_eq.
-  - inversion_clear H; cat.
-  - destruct (arrs _); [|discriminate].
-    destruct s, s; equalities.
-    equalities'; auto.
-    equalities'; auto.
-    equalities; [|discriminate].
-    inversion_clear H.
-    reflexivity.
-  - destruct (termD m y f1) eqn:?, (termD x m f2) eqn:?; try discriminate.
-    specialize (IHf1 _ _ _ Heqo).
-    specialize (IHf2 _ _ _ Heqo0).
-    inversion_clear H.
-    red in IHf1.
-    red in IHf2.
-    destruct (arrowsD m y (arrows f1)) eqn:?; [|contradiction].
-    destruct (arrowsD x m (arrows f2)) eqn:?; [|contradiction].
-    destruct (arrowsD x y (map (Left m f1 f2) (arrows f1) ++
-                           map (Right m f1 f2) (arrows f2))) eqn:?.
-      apply arrowsD_app in Heqo3.
-      equalities.
-      rewrite <- IHf1, <- IHf2, b0.
-      rewrite a in Heqo1.
-      rewrite a0 in Heqo2.
-      inversion_clear Heqo1.
-      inversion_clear Heqo2.
-      reflexivity.
-    admit.
-Admitted.
-
-Lemma termD_arrowsD_none x y f :
-  termD x y f = None ↔ arrowsD x y (arrows f) = None.
-Proof.
-  generalize dependent y.
-  generalize dependent x.
-  induction f.
-  - destruct (arrs _); auto.
-  - destruct (arrs _); auto.
-  - destruct (termD m y f1) eqn:?.
-      destruct (termD x m f2) eqn:?.
-        discriminate.
-  admit.
-Admitted.
-*)
-
-Fixpoint exprD (e : Expr) : Type :=
-  match e with
-  | Top           => True
-  | Bottom        => False
-  | Equiv x y f g => termD x y f ≈ termD x y g
-  (* | Not p         => exprD p -> False *)
-  | And p q       => exprD p ∧ exprD q
-  | Or p q        => exprD p + exprD q
-  | Impl p q      => exprD p -> exprD q
-  end.
-
 Fixpoint exprAD (e : Expr) : Type :=
   match e with
   | Top           => True
@@ -228,46 +130,13 @@ Proof.
   destruct (arrowsD_sound Heqo), p.
   rewrite e0; clear e0.
   rewrite H1 in Heqo; clear H1.
-  destruct (arrowsD_sound Heqo), p.
-  rewrite e1; clear e1.
-  red.
-  rewrite <- e, <- e0.
-  reflexivity.
-
-  induction f; simpl in *; repeat equalities.
-  - destruct g; simpl in *; repeat equalities.
-    + destruct (arrs a); [|contradiction].
-      destruct s, s; equalities; contradiction.
-    + destruct (arrowsD x x (map (Left m g1 g2) (arrows g1) ++
-                             map (Right m g1 g2) (arrows g2))) eqn:?;
-      [|contradiction].
-      admit.
-  - destruct g; simpl in *; repeat equalities.
-    + destruct (arrs a); auto.
-    + destruct (arrowsD _ _ _) eqn:?; [contradiction|].
-        admit.
-  - admit.
 Admitted.
 
 Lemma exprAD_sound (e : Expr) : exprAD e -> exprD e.
 Proof.
   destruct e; auto; intros.
   red in X; red.
-  apply arrowsD_sound; auto.
-Qed.
+  apply arrowsD_apply; auto.
+Abort.
 
 End Denote.
-
-(*
-Context {C : Category}.
-Variable x : C.
-Variables f g h : x ~> x.
-
-Definition objs := (fun _ : obj_idx => x).
-
-Eval simpl in @exprD C objs
-  (fun i => if Pos.eqb i 1 then Some (1; (1; f)) else
-            if Pos.eqb i 2 then Some (1; (1; g)) else Some (1; (1; h)))%positive
-  (Equiv 1 1 (@Compose 1 (@Morph 1) (@Compose 1 (@Morph 2) (@Morph 3)))
-             (@Compose 1 (@Compose 1 (@Morph 1) (@Morph 2)) (@Morph 3)))%positive.
-*)
