src/Expr.v
@@ -21,12 +21,9 @@ Section Expr.
 Definition obj_idx := positive.
 Definition arr_idx := positive.
 
-(* This describes the morphisms of a magmoid, which forms a quotient category
-   under denotation. *)
 Inductive Term : Set :=
   | Identity (o : obj_idx) : Term
   | Morph    (x y : obj_idx) (a : arr_idx) : Term
-  (* With induction-recursion, the [m] argument would be unnecessary. *)
   | Compose  (m : obj_idx) (f : Term) (g : Term) : Term.
 
 Function term_beq (f g : Term) : bool :=
@@ -48,116 +45,12 @@ Proof.
   f_equal; intuition.
 Qed.
 
-Function term_dom (e : Term) : obj_idx :=
-  match e with
-  | Identity x    => x
-  | Morph x _ _   => x
-  | Compose _ _ g => term_dom g
-  end.
-
-Function term_cod (e : Term) : obj_idx :=
-  match e with
-  | Identity y    => y
-  | Morph _ y _   => y
-  | Compose _ f _ => term_cod f
-  end.
-
 Fixpoint term_size (t : Term) : nat :=
   match t with
   | Identity _    => 1%nat
   | Morph _ _ _   => 1%nat
   | Compose _ f g => 1%nat + term_size f + term_size g
   end.
-
-(*
-Inductive NormalForm : obj_idx -> obj_idx -> Term -> Term -> Type :=
-  | NFIdentity : ∀ x, NormalForm x x (Identity x) (Identity x)
-  | NFMorph : ∀ x y f, NormalForm x y (Morph x y f) (Morph x y f)
-  | NFCompose_Id_Left : ∀ x y f f',
-      NormalForm x y f f' ->
-      NormalForm x y (Compose y (Identity y) f) f'
-  | NFCompose_Id_Right : ∀ x y f f',
-      NormalForm x y f f' ->
-      NormalForm x y (Compose x f (Identity x)) f'
-  | NFCompose_Morph : ∀ x y z f g g',
-      NormalForm y z g g' ->
-      NormalForm x z (Compose z (Morph y z f) g)
-                     (Compose z (Morph y z f) g')
-  | NFCompose_Assoc : ∀ x y z w f f' g g' h h',
-      NormalForm z w f f' ->
-      NormalForm y z g g' ->
-      NormalForm x y h h' ->
-      NormalForm x w (Compose y (Compose z f g) h)
-                     (Compose z f' (Compose y g' h')).
-
-Definition term_append (t : Term) : ∃ t' x y, NormalForm x y t t'.
-Proof.
-  induction t.
-  - do 3 eexists; econstructor.
-  - do 3 eexists; econstructor.
-  - equalities.
-    destruct t1; simpl.
-    + inversion n0; subst.
-      exists t2, o, o.
-      apply NFCompose_Id_Left.
-      admit.
-    + exists (Compose m (Morph x1 y a) t2).
-      admit.
-    + exists (Compose m0 t1_1 (Compose m t1_2 t2)).
-      constructor.
-
-Program Fixpoint term_append (t u : Term) :
-  ∃ t' m, NormalForm (Compose m t u) t'  :=
-  match t with
-  | Compose m g h =>
-    match term_append h u with
-    | (t'; (u'; h')) => _ term_append g t'
-    end
-  | Identity o    => _ u
-  | Morph x y a   =>
-    match u with
-    | Identity _ => _ t
-    | _ => _ (Compose x t u)
-    end
-  end.
-Next Obligation.
-  eexists; eexists.
-  econstructor; eauto.
-*)
-
-Function term_append (t u : Term) : Term :=
-  match t with
-  | Compose m g h => term_append g (term_append h u)
-  | Identity _    => u
-  | Morph x y a   =>
-    match u with
-    | Identity _ => t
-    | _ => Compose x t u
-    end
-  end.
-
-Functional Scheme term_append_scheme :=
-  Induction for term_append Sort Type.
-
-Definition term_normal (t : Term) : Term :=
-  term_append t (Identity (term_dom t)).
-
-Definition term_equiv (f g : Term) := term_normal f = term_normal g.
-
-Example normalize_term_ex1 :
-  term_normal
-    (Compose
-       1 (Compose
-            1 (Compose 1 (Morph 1 1 1) (Identity 1))
-              (Compose 1 (Morph 1 1 3) (Morph 1 1 4)))
-         (Compose
-            1 (Compose 1 (Identity 1) (Identity 1))
-              (Compose 1 (Morph 1 1 7) (Morph 1 1 8))))%positive
-    = (Compose 1 (Morph 1 1 1)
-         (Compose 1 (Morph 1 1 3)
-            (Compose 1 (Morph 1 1 4)
-               (Compose 1 (Morph 1 1 7) (Morph 1 1 8)))))%positive.
-Proof. reflexivity. Qed.
 
 Inductive Expr : Set :=
   | Top
